Common/Exec.v
@@ -44,7 +44,11 @@
 
 (** This file defines an execution monad for operational models.
 
-This monad supports non determinism and errors. Use StateT to add state. *)
+    This monad supports states, non determinism, and errors.
+    As an intermediate step the [res] monad is defined,
+    that supports non-determinism and errors.
+    The definition of the execution monad then makes use of [res] and its
+    monadic functions, and adds states to both valid results and errors *)
 
 Require Import Options.
 Require Import Common.
@@ -54,88 +58,181 @@ Require Import Effects.
 (* TODO: Make it a top level name *)
 Module Exec.
 
-(** * Base definitions *)
-Record t {E A : Type} := make {
+(** * Base execution result definitions *)
+Record res {E A : Type} := make {
     results: list A;
     errors: list E;
   }.
-Arguments t : clear implicits.
+Arguments res : clear implicits.
 Arguments make {_ _}.
 
-(** Decide if a execution has errors *)
-Definition has_error `(e : t E A) :=
+(** Decide if a result has errors *)
+Definition has_error `(e : res E A) :=
   match e with
   | make _ [] => False
   | _ => True
   end.
-#[global] Instance has_error_dec `(e : t E A): Decision (has_error e).
+#[global] Instance has_error_dec `(e : res E A): Decision (has_error e).
 Proof. unfold_decide. Qed.
+
+(** Merge two execution results by merging successes and errors separately.
+    This does not perform de-duplication *)
+Definition merge {E A} (er1 er2 : res E A) :=
+  make (er1.(results) ++ er2.(results)) (er1.(errors) ++ er2.(errors)).
+#[export] Typeclasses Opaque merge.
+Arguments merge : simpl never.
+
+(** Create a res record from a set of results, e.g. to convert from pure
+    non-determinism to res *)
+Definition res_Results {E A C} `{Elements A C} (s : C) : res E A :=
+  make (elements s) [].
+
+(** Monadic definitions for executions results *)
+
+#[global] Instance res_mret_inst {E} : MRet (res E) := λ _ v, make [v] [].
+
+#[global] Instance res_mbind_inst {E} : MBind (res E) :=
+  λ _ _ f e,
+    foldr merge (make [] e.(errors)) (map f e.(results)).
+#[global] Typeclasses Opaque res_mbind_inst.
+
+#[global] Instance res_fmap_inst {E} : FMap (res E) :=
+  λ _ _ f e, make (map f e.(results)) e.(errors).
+#[global] Typeclasses Opaque res_fmap_inst.
+
+#[global] Instance res_throw_inst {E} : MThrow E (res E) :=
+  λ _ e, make [] [e].
+
+#[global] Instance res_choose_inst {E} : MChoose (res E) :=
+  λ '(ChooseFin n), @res_Results  _ (Fin.t n) _ _ (enum (fin n)).
+
+(** Convert an execution result into a list of results *)
+Definition to_result_list `(e : res E A) : list (result E A) :=
+  map Ok e.(results) ++ map Error e.(errors).
+
+(** Convert an execution result with states into a list of results *)
+Definition to_stateful_result_list `(e : res (St * E) (St * A)) :
+    list (St * result E A) :=
+  map (λ '(st,r), (st, Ok r)) e.(results) ++ map (λ '(st,err), (st, Error err))
+      e.(errors).
+
+(** Convert an execution result into a list of result states *)
+Definition to_state_result_list `(e : res (St * E) (St * A)) :
+    list (result St St) :=
+  map (Ok ∘ fst) e.(results) ++ map (Error ∘ fst) e.(errors).
+
+(** Convert and execution result into a list of successful states *)
+Definition success_state_list `(e : res (St * E) (St * A)) : list St :=
+  e.(results).*1.
+
+(** * Base execution monad definitions *)
+
+Definition t {St E A} := St → res (St * E) (St * A).
+Arguments t : clear implicits.
+#[export] Typeclasses Transparent t.
 
 (** Create an execution from a set of results, e.g. to convert from pure
     non-determinism to Exec *)
-Definition Results {E A C} `{Elements A C} (s : C) : t E A := make (elements s) [].
+Definition Results {St E A C} `{Elements A C} (s : C) : t St E A :=
+  λ st, (st,.) <$> res_Results s.
 
-(** Merge the results of two executions *)
-Definition merge {E A} (e1 e2 : t E A) :=
-  make (e1.(results) ++ e2.(results)) (e1.(errors) ++ e2.(errors)).
-#[global] Typeclasses Opaque merge.
-Arguments merge : simpl never.
+(** Monadic definition based on the respective instances for execution results *)
 
-(** Convert an execution into a list of results *)
-Definition to_result_list `(e : t E A) : list (result E A) :=
-  map Ok e.(results) ++ map Error e.(errors).
+#[global] Instance mret_inst {St E} : MRet (t St E) := λ _ v st, mret (st,v).
 
-#[global] Instance mret_inst {E} : MRet (t E) := λ _ v, make [v] [].
-
-#[global] Instance mbind_inst {E} : MBind (t E) :=
-  λ _ _ f e, foldr merge (make [] e.(errors)) (map f e.(results)).
+#[global] Instance mbind_inst {St E} : MBind (t St E) :=
+  λ _ _ f e st, '(st', a) ← e st; f a st'.
 #[global] Typeclasses Opaque mbind_inst.
 
-#[global] Instance fmap_inst {E} : FMap (t E) :=
-  λ _ _ f e, make (map f e.(results)) e.(errors).
+#[global] Instance fmap_inst {St E} : FMap (t St E) :=
+  λ _ _ f e st, (λ '(st',a), (st', f a)) <$> e st.
 #[global] Typeclasses Opaque fmap_inst.
 
-#[global] Instance throw_inst {E} : MThrow E (t E) := λ _ e, make [] [e].
+#[global] Instance throw_inst {St E} : MThrow E (t St E) :=
+  λ _ e st, mthrow (st,e).
 
-#[global] Instance choose_inst {E} : MChoose (t E) :=
-  λ '(ChooseFin n), make (enum (fin n)) [].
+#[global] Instance choose_inst {St E} : MChoose (t St E) :=
+  λ '(ChooseFin n), @Results _ _ (Fin.t n) _ _ (enum (fin n)).
+
 #[global] Typeclasses Opaque choose_inst.
 
-Lemma mdiscard_eq {E A} : mdiscard =@{t E A} make [] [].
+#[global] Instance st_call_MState {St E} : MCall (MState St) (t St E) | 10 :=
+  λ eff,
+    match eff with
+    | MSet s => λ _, make [(s,())] []
+    | MGet => λ s, make [(s,s)] []
+    end.
+
+Lemma mdiscard_eq {St E A} : mdiscard =@{t St E A} (λ st, make [] []).
 Proof. reflexivity. Qed.
 
-#[global] Instance elem_of_results {E A} : ElemOf A (t E A) :=
-  λ x e, x ∈ e.(results).
+Definition map_state `(f : St → St') `(r : res (St * E) (St * A)) :
+    res (St' * E) (St' * A) :=
+  make (map (λ '(st, a), (f st, a)) r.(results))
+       (map (λ '(st, a), (f st, a)) r.(errors)).
+
+Definition liftSt_full {St St' E A} (getter : St → St') (setter : St' → St → St)
+    (inner : Exec.t St' E A) : Exec.t St E A :=
+  λ st, map_state (λ st', setter st' st) (inner (getter st)).
+
+Definition liftSt {St St' E A} (getter : St → St') `{Setter St St' getter}
+    (inner : Exec.t St' E A) : Exec.t St E A :=
+  liftSt_full getter (@setv _ _ getter _) inner.
+
+Definition lift_res_set_full {St' St} (setter : St' → St → St)
+    `(r : res (St' * E) (St' * A)) : t St E A :=
+  λ st, map_state (λ st', setter st' st) r.
+
+Definition lift_res_set {St' St} (getter : St → St') `{Setter St St' getter}
+    `(r : res (St' * E) (St' * A)) : t St E A :=
+  lift_res_set_full (@setv _ _ getter _) r.
+
+#[global] Instance elem_of_results {E A} : ElemOf A (res E A) :=
+  λ x r, x ∈ r.(results).
 #[global] Typeclasses Opaque elem_of_results.
 
-#[global] Instance elem_of_result {E A} : ElemOf (result E A) (t E A) :=
+#[global] Instance elem_of_results_no_state {St E A} :
+    ElemOf A (res (St * E) (St * A)) :=
+  λ x r, x ∈ (map snd r.(results)).
+#[global] Typeclasses Opaque elem_of_results_no_state.
+
+
+#[global] Instance elem_of_result {E A} : ElemOf (result E A) (res E A) :=
   λ x e, match x with
          | Ok v => v ∈ e
          | Error err => err ∈ e.(errors)
          end.
 #[global] Typeclasses Opaque elem_of_result.
 
+#[global] Instance elem_of_result_no_state {St E A} :
+    ElemOf (result E A) (res (St * E) (St * A)) :=
+  λ x e, match x with
+         | Ok v => v ∈ e
+         | Error err => err ∈ (snd <$> e.(errors))
+         end.
+#[global] Typeclasses Opaque elem_of_result.
+
 (** Takes an option but convert None into an error *)
-Definition error_none {E A} (e : E) : option A -> t E A :=
+Definition error_none {St E A} (e : E) : option A -> t St E A :=
   from_option mret (mthrow e).
 
 (** Takes an option but convert None into a discard *)
-Definition discard_none {E A} : option A -> t E A :=
+Definition discard_none {St E A} : option A -> t St E A :=
   from_option mret mdiscard.
 
 (** Maps the error to another error type. *)
-Definition map_error {E E' A} (f : E -> E') (e : t E A) : t E' A :=
-  make e.(results) (map f e.(errors)).
-(** Merge the results of two executions *)
+Definition map_error {St E E' A} (f : E -> E') (e : t St E A) : t St E' A :=
+  λ st, let est := e st in
+    make est.(results) (map (λ '(st', r), (st', f r)) est.(errors)).
 
-(** * Unfold typeclass for results *)
+(** * Unfold typeclass for execution results *)
 
-Class UnfoldElemOf {A E} (x : A) (e : t E A) (Q : Prop) :=
+Class UnfoldElemOf {A E} (x : A) (e : res E A) (Q : Prop) :=
   {unfold_elem_of : x ∈ e ↔ Q}.
 #[global] Hint Mode UnfoldElemOf + + - + - : typeclass_instances.
 
-#[global] Instance unfold_elem_of_default {A E} (x : A) (e : t E A) :
-  UnfoldElemOf x e (x ∈ e) | 1000.
+#[global] Instance unfold_elem_of_default {A E} (x : A) (r : res E A) :
+  UnfoldElemOf x r (x ∈ r) | 1000.
 Proof. done. Qed.
 
 #[export] Hint Extern 5 (UnfoldElemOf ?x (match ?b with _ => _ end) ?G) =>
@@ -152,7 +249,7 @@ Proof. done. Qed.
   destruct b; cbn zeta match : typeclass_instances.
 
 #[global] Instance UnfoldElemOf_proper {A E} :
-  Proper (@eq A ==> @eq (t E A) ==> iff ==> iff) UnfoldElemOf.
+  Proper (@eq A ==> @eq (res E A) ==> iff ==> iff) UnfoldElemOf.
 Proof. solve_proper2_tc. Qed.
 
 (** Enables Exec unfolding in regular set_unfold *)
@@ -167,75 +264,114 @@ Proof. tcclean. apply unfold_elem_of. Qed.
 
 (** ** Actual unfolding lemmas *)
 
-#[global] Instance unfold_elem_of_make {E A} x l l' P:
-  SetUnfoldElemOf x l P →
-  UnfoldElemOf x (make l l' : t E A) P.
+#[global] Instance unfold_elem_of_results {E A} x (e : res E A) P:
+  UnfoldElemOf x e P →
+  SetUnfoldElemOf x e.(results) P | 1000.
 Proof. tcclean. naive_solver. Qed.
 
-#[global] Instance unfold_elem_of_mret {E A} x y:
-  UnfoldElemOf x (mret y : t E A) (x = y).
-Proof. tcclean. unfold mret, mret_inst. set_solver. Qed.
+#[global] Instance unfold_elem_of_make {E A} x l l' P:
+  SetUnfoldElemOf x l P →
+  UnfoldElemOf x (make l l' : res E A) P.
+Proof. tcclean. naive_solver. Qed.
 
-#[global] Instance unfold_elem_of_merge {E A} x (e e' : t E A) P Q:
+#[global] Instance unfold_elem_of_mret {St E A} st x y:
+  UnfoldElemOf x ((mret y : t St E A) st) (x = (st, y)).
+Proof. tcclean. do 2 unfold mret, mret_inst, res_mret_inst. set_solver. Qed.
+
+#[global] Instance unfold_elem_of_merge {E A} x (e e' : res E A) P Q :
   UnfoldElemOf x e P →
   UnfoldElemOf x e' Q →
   UnfoldElemOf x (merge e e') (P ∨ Q).
 Proof. tcclean. unfold merge. destruct e. destruct e'. set_solver. Qed.
 
-#[global] Instance unfold_elem_of_mbind {E A B} (x : B) (e : t E A) (f : A → t E B) P:
+#[global] Instance unfold_elem_of_mbind {St E A B} st (x : St * B) (e : t St E A)
+    (f : A → t St E B) P :
+  (∀ y, UnfoldElemOf y (e st) (P y)) →
+  UnfoldElemOf x ((e ≫= f) st) (∃ st' y, P (st', y) ∧ x ∈ f y st') | 20.
+Proof.
+  tcclean. deintro. intros _.
+  unfold mbind, mbind_inst.
+  destruct (e st) as [l es].
+  elim l; cdestruct |- ***; set_solver.
+Qed.
+
+#[global] Instance unfold_elem_of_bind_guard `{Decision P} {St E A} st
+    (e : t St E A) (err : E) a Q :
+  UnfoldElemOf a (e st) Q →
+  UnfoldElemOf a ((guard_or err P;; e) st) (P ∧ Q) | 10.
+Proof. tcclean. case_guard; set_solver. Qed.
+
+#[global] Instance unfold_elem_of_bind_guard_discard `{Decision P} {St E A} st
+    (e : t St E A) a Q :
+  UnfoldElemOf a (e st) Q →
+  UnfoldElemOf a ((guard_discard P;; e) st) (P ∧ Q) | 10.
+Proof. tcclean. case_guard_discard; set_solver. Qed.
+
+#[global] Instance unfold_elem_of_fmap {St E A B} st (x : St * B) (e : t St E A)
+    (f : A → B) P :
+  (∀ p, UnfoldElemOf p (e st) (P p)) →
+  UnfoldElemOf x ((f <$> e) st) (∃ st' y, P (st', y) ∧ x = (st', f y)).
+Proof. tcclean. unfold elem_of, elem_of_results, fmap, fmap_inst.
+  destruct (e st) as [l es]. cbn. set_unfold.
+  cdestruct |- *** #CDestrSplitGoal; repeat eexists; eauto; naive_solver.
+Qed.
+
+#[global] Instance unfold_elem_of_mdiscard {St E A} st (x : St * A) :
+  UnfoldElemOf x ((mdiscard : t St E A) st) False.
+Proof. tcclean. unfold mdiscard, fmap, fmap_inst; cbn. set_solver. Qed.
+
+#[global] Instance unfold_elem_of_Results {St E A C} `{Elements A C} (s : C)
+    (x : St * A) st P :
+  (∀ y : A, SetUnfoldElemOf y (elements s) (P y)) →
+  UnfoldElemOf x (Results (E := E) s st) (P x.2 ∧ x.1 = st).
+Proof. tcclean. unfold Results, res_Results. destruct x. cbn. set_solver. Qed.
+
+#[global] Instance unfold_elem_of_mcallM_MChoice {St E} st st' (m : MChoice)
+    (v : eff_ret m) :
+  UnfoldElemOf (st, v) (mcallM (Exec.t St E) m st') (st = st').
+Proof.
+  tcclean.
+  destruct m.
+  cbn -[enum] in *.
+  unfold mcallM, choose_inst, enum.
+  destruct fin_finite.
+  set_solver.
+Qed.
+
+#[global] Instance res_unfold_elem_of_mbind {E A B} (x :  B) (e : res E A) (f : A → res E B) P:
   (∀ y, UnfoldElemOf y e (P y)) →
   UnfoldElemOf x (e ≫= f) (∃ y, P y ∧ x ∈ f y) | 20.
 Proof.
-  tcclean. deintro. intros _. destruct e as [l es]. cbn.
-  setoid_rewrite unfold_elem_of.
-  induction l; set_solver.
+  tcclean. deintro. intros _.
+  unfold mbind, res_mbind_inst.
+  destruct e as [l es].
+  elim l; cdestruct |- ***; set_solver.
 Qed.
-
-#[global] Instance unfold_elem_of_bind_guard `{Decision P} {E A} (e : t E A)
-    (err : E) a Q:
-  UnfoldElemOf a e Q →
-  UnfoldElemOf a (guard_or err P;; e) (P ∧ Q) | 10.
-Proof. tcclean. case_guard; set_solver. Qed.
-
-#[global] Instance unfold_elem_of_bind_guard_discard `{Decision P} {E A} (e : t E A) a Q:
-  UnfoldElemOf a e Q →
-  UnfoldElemOf a (guard_discard P;; e) (P ∧ Q) | 10.
-Proof. tcclean. case_guard_discard; set_solver. Qed.
-
-#[global] Instance unfold_elem_of_fmap {E A B} (x : B) (e : t E A) (f : A → B) P:
-  (∀ y, UnfoldElemOf y e (P y)) →
-  UnfoldElemOf x (f <$> e) (∃ y, P y ∧ x = f y).
-Proof. tcclean. destruct e as [l es]. cbn. set_solver. Qed.
-
-#[global] Instance unfold_elem_of_mdiscard {E A} (x : A) :
-  UnfoldElemOf x (mdiscard : t E A) False.
-Proof. tcclean. unfold mdiscard. set_solver. Qed.
-
 
 (** * Unfold the [has_error] predicate *)
 
-Class UnfoldHasError `(e : t E A) (Q : Prop) :=
+Class UnfoldHasError `(e : res E A) (Q : Prop) :=
   {unfold_has_error : has_error e ↔ Q }.
 #[global] Hint Mode UnfoldHasError + + + - : typeclass_instances.
 
-#[global] Instance unfold_has_error_default `(e : t E A) :
+#[global] Instance unfold_has_error_default `(e : res E A) :
   UnfoldHasError e (has_error e) | 1000.
 Proof. done. Qed.
 
-#[global] Instance unfold_has_error_mret {E A} (x : A):
-  UnfoldHasError (mret x: t E A) False.
+#[global] Instance unfold_has_error_mret {St E A} st (x : A) :
+  UnfoldHasError ((mret x : t St E A) st) False.
 Proof. done. Qed.
 
-#[global] Instance unfold_has_error_mthrow {E A} (err : E):
-  UnfoldHasError (mthrow err: t E A) True.
+#[global] Instance unfold_has_error_mthrow {St E A} st (err : E) :
+  UnfoldHasError ((mthrow err: t St E A) st) True.
 Proof. done. Qed.
 
-#[global] Instance unfold_has_error_mdiscard {E A}:
-  UnfoldHasError (mdiscard: t E A) False.
+#[global] Instance unfold_has_error_mdiscard {St E A} st :
+  UnfoldHasError ((mdiscard: t St E A) st) False.
 Proof. done. Qed.
 
 
-#[global] Instance unfold_has_error_merge {E A} (e e' : t E A) P Q:
+#[global] Instance unfold_has_error_merge {E A} (e e' : res E A) P Q :
   UnfoldHasError e P →
   UnfoldHasError e' Q →
   UnfoldHasError (merge e e') (P ∨ Q).
@@ -244,37 +380,41 @@ Proof.
   destruct e as [ ? []]; destruct e' as [? []]; cbn in *; naive_solver.
 Qed.
 
-#[global] Instance unfold_has_error_mbind {E A B} (e : t E A) (f : A → t E B) P Q R:
-  UnfoldHasError e P →
-  (∀ y, UnfoldElemOf y e (Q y)) →
-  (∀ y, UnfoldHasError (f y) (R y)) →
-  UnfoldHasError (e ≫= f) (P ∨ ∃ y, Q y ∧ R y) | 20.
+#[global] Instance unfold_has_error_mbind {St E A B} st (e : t St E A)
+    (f : A → t St E B) P Q R :
+  UnfoldHasError (e st) P →
+  (∀ y, UnfoldElemOf y (e st) (Q y)) →
+  (∀ y, UnfoldHasError (f y.2 y.1) (R y)) →
+  UnfoldHasError ((e ≫= f) st) (P ∨ ∃ y, Q y ∧ R y) | 20.
 Proof.
   tcclean.
   clear H.
   clear H1.
   clear H0.
-  destruct e as [l e]; cbn.
+  unfold mbind, mbind_inst.
+  destruct (e st) as [l es]; cbn.
   setoid_rewrite unfold_elem_of.
-  induction l.
+  induction l as [|[]].
   - set_solver.
   - cbn. rewrite unfold_has_error. set_solver.
 Qed.
 
-#[global] Instance unfold_has_error_bind_guard `{Decision P} {E A} (e : t E A)
-  (err : E) Q:
-  UnfoldHasError e Q →
-  UnfoldHasError (guard_or err P;; e) (¬ P ∨ Q) | 10.
+#[global] Instance unfold_has_error_bind_guard `{Decision P} {St E A} st
+  (e : t St E A) (err : E) Q :
+  UnfoldHasError (e st) Q →
+  UnfoldHasError ((guard_or err P;; e) st) (¬ P ∨ Q) | 10.
 Proof. tcclean. case_guard; try rewrite unfold_has_error; naive_solver. Qed.
 
-#[global] Instance unfold_has_error_bind_guard_discard `{Decision P} {E A} (e : t E A) Q:
-  UnfoldHasError e Q →
-  UnfoldHasError (guard_discard P;; e) (P ∧ Q) | 10.
+#[global] Instance unfold_has_error_bind_guard_discard `{Decision P} {St E A} st
+    (e : t St E A) Q :
+  UnfoldHasError (e st) Q →
+  UnfoldHasError ((guard_discard P;; e) st) (P ∧ Q) | 10.
 Proof. tcclean. case_guard_discard; try rewrite unfold_has_error; naive_solver. Qed.
 
-#[global] Instance unfold_has_error_fmap {E A B} (e : t E A) (f : A → B) P:
-  UnfoldHasError e P →
-  UnfoldHasError (f <$> e) P.
-Proof. tcclean. destruct e as [l es]. cbn. set_solver. Qed.
+#[global] Instance unfold_has_error_fmap {St E A B} st (e : t St E A) (f : A → B) P :
+  UnfoldHasError (e st) P →
+  UnfoldHasError ((f <$> e) st) P.
+Proof. tcclean. unfold fmap, fmap_inst. destruct (e st) as [l es]. easy. Qed.
 
 End Exec.
+
