Common/CDestruct.v
@@ -291,6 +291,9 @@ Global Hint Extern 3 (ObvTrue _) =>
 Global Hint Extern 4 (ObvTrue _) =>
          constructor; symmetry; assumption : typeclass_instances.
 
+#[global] Instance obv_true_not_False : ObvTrue (¬ False).
+Proof. now tcclean. Qed.
+
 (** * CDestruct
 
 See the top of the file comment for details about what [cdestruct] does. *)
@@ -882,4 +885,20 @@ Proof. tcclean. tauto. Qed.
 
 Instance cdestruct_not_or_and b P Q :
   CDestrSimpl b (¬ (P ∨ Q)) (¬ P ∧ ¬ Q).
+Proof. tcclean. naive_solver. Qed.
+
+Instance cdestruct_or_False_l b P :
+  CDestrSimpl b (False ∨ P) P.
+Proof. tcclean. naive_solver. Qed.
+
+Instance cdestruct_or_False_r b P :
+  CDestrSimpl b (P ∨ False) P.
+Proof. tcclean. naive_solver. Qed.
+
+Instance cdestruct_and_True_l b P :
+  CDestrSimpl b (True ∧ P) P.
+Proof. tcclean. naive_solver. Qed.
+
+Instance cdestruct_and_True_r b P :
+  CDestrSimpl b (P ∧ True) P.
 Proof. tcclean. naive_solver. Qed.
